Refactor stack recombination, add cons lemmas
Add a stack-based definition to the existing state-based one, and
reformulate the latter in terms of the former. This, in combination with
the rewrite lemmas on merged states, makes exposing the structure of the
recombined states easier.

In addition to those results, state lemmas to expose the top of a merged
stack based on program vs. context information, determining which state
to select from.

Intermediate/Recombination.v
@@ -376,12 +376,15 @@ Section Merge.
      and memories "without holes" w.r.t. to the generating states and interfaces,
      provided that the mergeability assumptions is present. *)
 
-  (* RB: TODO: Rename these definitions to merge_states_. *)
-  Definition mergeable_states_stack (s s'' : CS.state) : CS.stack :=
+  Definition merge_stacks (gps gps'' : CS.stack) : CS.stack :=
     PS.unpartialize_stack
       (PS.merge_stacks
-         (PS.to_partial_stack (CS.state_stack s  ) (domm ic))
-         (PS.to_partial_stack (CS.state_stack s'') (domm ip))).
+         (PS.to_partial_stack gps (domm ic))
+         (PS.to_partial_stack gps'' (domm ip))).
+
+  (* RB: TODO: Rename these definitions to merge_states_. *)
+  Definition mergeable_states_stack (s s'' : CS.state) : CS.stack :=
+    merge_stacks (CS.state_stack s) (CS.state_stack s'').
 
   Definition merge_memories (mem mem'' : Memory.t) : Memory.t :=
     PS.merge_memories
@@ -413,6 +416,18 @@ Section Merge.
 
   (* RB: TODO: Add side conditions (well-formed programs, linkable interfaces,
      etc. *)
+  Lemma merge_stacks_cons_program frame gps frame'' gps'' :
+    Pointer.component frame \in domm ip ->
+    merge_stacks (frame :: gps) (frame'' :: gps'') =
+    frame :: merge_stacks gps gps''.
+  Admitted.
+
+  Lemma merge_stacks_cons_context frame gps frame'' gps'' :
+    Pointer.component frame \in domm ic ->
+    merge_stacks (frame :: gps) (frame'' :: gps'') =
+    frame'' :: merge_stacks gps gps''.
+  Admitted.
+
   Lemma mergeable_states_merge s s'' :
     mergeable_states s s'' ->
     merge_states s s'' =
@@ -427,6 +442,16 @@ Section Merge.
      mergeable_states_memory s s'',
      state_regs s,
      CS.state_pc s).
+  Admitted.
+
+  Lemma mergeable_states_merge_context s s'' :
+    CS.is_context_component s ic ->
+    mergeable_states s s'' ->
+    merge_states s s'' =
+    (mergeable_states_stack s s'',
+     mergeable_states_memory s s'',
+     state_regs s'',
+     CS.state_pc s'').
   Admitted.
 
   Lemma mergeable_states_pc_same_component s s'' :
